RISC-V: handle mem exceptions, drop dummy alignment check

case_study/RiscvPmp/Types.v
@@ -148,6 +148,12 @@ Inductive FetchResult : Set :=
 | F_Error (e : ExceptionType) (v : Word)
 .
 
+(* NOTE: simplified to only take the ctl_trap constructor into account
+         (other constructors are for mret, sret and uret, not considered atm) *)
+Inductive CtlResult : Set :=
+| CTL_TRAP (e : ExceptionType)
+.
+
 Inductive ASTConstructor : Set :=
 | KRTYPE
 | KITYPE
@@ -182,12 +188,17 @@ Inductive FetchResultConstructor : Set :=
 | KF_Error
 .
 
+Inductive CtlResultConstructor : Set :=
+| KCTL_TRAP
+.
+
 Inductive Unions : Set :=
 | ast
 | access_type
 | exception_type
 | memory_op_result
 | fetch_result
+| ctl_result
 .
 
 Record Pmpcfg_ent : Set :=
@@ -229,6 +240,8 @@ Section TransparentObligations.
   Derive NoConfusion for MemoryOpResultConstructor.
   Derive NoConfusion for FetchResult.
   Derive NoConfusion for FetchResultConstructor.
+  Derive NoConfusion for CtlResult.
+  Derive NoConfusion for CtlResultConstructor.
   Derive NoConfusion for Records.
   Derive NoConfusion for Pmpcfg_ent.
 End TransparentObligations.
@@ -256,6 +269,8 @@ Derive EqDec for MemoryOpResult.
 Derive EqDec for MemoryOpResultConstructor.
 Derive EqDec for FetchResult.
 Derive EqDec for FetchResultConstructor.
+Derive EqDec for CtlResult.
+Derive EqDec for CtlResultConstructor.
 Derive EqDec for Records.
 Derive EqDec for Pmpcfg_ent.
 
@@ -415,6 +430,16 @@ Section Finite.
   Next Obligation.
     intros []; apply elem_of_list_In; cbn; intuition.
   Qed.
+
+  Global Program Instance CtlResultConstructor_finite :
+    Finite CtlResultConstructor :=
+    {| enum := [KCTL_TRAP] |}.
+  Next Obligation.
+    now apply nodup_fixed.
+  Qed.
+  Next Obligation.
+    intros []; apply elem_of_list_In; cbn; intuition.
+  Qed.
 End Finite.
 
 Module RiscvPmpTypeKit <: TypeKit.
@@ -452,6 +477,7 @@ Module RiscvPmpTypeKit <: TypeKit.
     | exception_type   => ExceptionType
     | memory_op_result => MemoryOpResult
     | fetch_result     => FetchResult
+    | ctl_result       => CtlResult
     end.
   Instance 𝑼𝑻_eq_dec U : EqDec (𝑼𝑻 U) :=
     ltac:(destruct U; cbn; auto with typeclass_instances).
@@ -463,6 +489,7 @@ Module RiscvPmpTypeKit <: TypeKit.
     | exception_type   => ExceptionTypeConstructor
     | memory_op_result => MemoryOpResultConstructor
     | fetch_result     => FetchResultConstructor
+    | ctl_result       => CtlResultConstructor
     end.
   Instance 𝑼𝑲_eq_dec U : EqDec (𝑼𝑲 U) :=
     ltac:(destruct U; auto with typeclass_instances).
